Doesn't build yet, but a slew of changes to incorporate the new whizzy function definition principle for definitions over binders.

examples/lambda/NEWLib.sml
@@ -1,0 +1,62 @@
+structure NEWLib :> NEWLib =
+struct
+
+open HolKernel Parse boolLib BasicProvers simpLib
+open ncTheory
+
+val FRESH_STRING = prove(
+  ``!X Y. FINITE (X:string set) /\ Y SUBSET X ==> ~(NEW X IN Y)``,
+  PROVE_TAC [pred_setTheory.SUBSET_DEF, dBTheory.NEW_FRESH_string]);
+
+val FRESH_STRING_eq = prove(
+  ``!X x. FINITE (X:string set) /\ x IN X ==> ~(NEW X = x)``,
+  PROVE_TAC [pred_setTheory.SUBSET_DEF, dBTheory.NEW_FRESH_string]);
+
+fun NEW_TAC vname t = let
+  val var = mk_var(vname, ``:string``)
+  val new_t = mk_comb(``NEW:string set -> string``, t)
+  val asm = mk_eq(var, new_t)
+  fun union_inds (sets, inds) t = let
+    val (f, args) = strip_comb t
+  in
+    if same_const f pred_setSyntax.union_tm then
+      union_inds (union_inds (sets, inds) (hd args)) (hd (tl args))
+    else if same_const f pred_setSyntax.insert_tm then
+      union_inds (sets, hd args::inds) (hd (tl args))
+    else if same_const f pred_setSyntax.empty_tm then (sets, inds)
+    else (t::sets, inds)
+  end
+  val (sets, inds) = union_inds ([], []) t
+  val munge = UNDISCH o CONV_RULE (LAND_CONV (ONCE_REWRITE_CONV [EQ_SYM_EQ]))
+  fun mk_IN (v,s) = let
+    val ty = type_of v
+  in
+    list_mk_comb(inst [alpha |-> ty] pred_setSyntax.in_tm, [v,s])
+  end
+  fun prove_ind i =
+      munge (SIMP_PROVE (srw_ss()) [FRESH_STRING_eq]
+                        (mk_imp(asm, mk_neg(mk_eq(var, i)))))
+  fun prove_set s =
+      munge (prove(mk_imp(asm, mk_neg(mk_IN(var, s))),
+                   DISCH_THEN SUBST_ALL_TAC THEN
+                   MATCH_MP_TAC FRESH_STRING THEN
+                   SIMP_TAC (srw_ss()) [pred_setTheory.SUBSET_DEF]))
+in
+  Q.ABBREV_TAC `^asm` THEN
+  MAP_EVERY (ASSUME_TAC o prove_ind) inds THEN
+  MAP_EVERY (ASSUME_TAC o prove_set) sets THEN
+  FIRST_X_ASSUM (K ALL_TAC o assert (is_eq o concl))
+end
+
+(* ----------------------------------------------------------------------
+    NEW_ELIM_TAC
+   ---------------------------------------------------------------------- *)
+
+fun NEW_ELIM_TAC (asl, w) = let
+  val newt = find_term (can (match_term ``NEW (X:string set)``)) w
+in
+  CONV_TAC (UNBETA_CONV newt) THEN MATCH_MP_TAC NEW_ELIM_RULE THEN
+  SIMP_TAC (srw_ss()) [FINITE_FV]
+end (asl, w)
+
+end (* struct *)
