examples/lambda/ncLib.sig
@@ -8,6 +8,6 @@ sig
   val recursive_term_function_existence : term -> thm
   val prove_recursive_term_function_exists : term -> thm
   val define_recursive_term_function :
-      term quotation -> thm * (thm * thm) option
+      term quotation -> thm * thm option
 
 end;
