examples/lambda/swapScript.sml
@@ -4,7 +4,7 @@ open simpLib boolSimps bossLib BasicProvers metisLib
 
 val _ = new_theory "swap"
 
-open ncTheory ncLib pred_setTheory chap2Theory
+open ncTheory NEWLib pred_setTheory
 
 (* ----------------------------------------------------------------------
     Basic swapping on strings
@@ -49,10 +49,39 @@ in
 end (asl, g)
 val swapstr_swapstr = store_thm(
   "swapstr_swapstr",
-  ``swapstr x y (swapstr u v s) =
-    swapstr (swapstr x y u) (swapstr x y v) (swapstr x y s)``,
+  ``swapstr (swapstr x y u) (swapstr x y v) (swapstr x y s) =
+    swapstr x y (swapstr u v s)``,
   REWRITE_TAC [swapstr_def] THEN
   REPEAT simp_cond_tac);
+val _ = export_rewrites ["swapstr_swapstr"]
+
+val swapstr_swapstr2 = store_thm(
+  "swapstr_swapstr2",
+  ``swapstr x y (swapstr (swapstr x y a) (swapstr x y b) s) =
+    swapstr a b (swapstr x y s)``,
+  CONV_TAC (LAND_CONV (ONCE_REWRITE_CONV [GSYM swapstr_swapstr])) THEN
+  REWRITE_TAC [swapstr_inverse]);
+val _ = export_rewrites ["swapstr_swapstr2"]
+
+val swapstr_eq_normalise = store_thm(
+  "swapstr_eq_normalise",
+  ``(s = swapstr x y t) = (swapstr x y s = t)``,
+  SRW_TAC [][swapstr_def] THEN PROVE_TAC []);
+val _ = export_rewrites ["swapstr_eq_normalise"]
+
+val swapstr_identity = store_thm(
+  "swapstr_identity",
+  ``~(x = s) /\ ~(y = s) ==>
+    (swapstr x y s = s) /\ ((swapstr x y t = s) = (t = s))``,
+  SRW_TAC [][swapstr_def]);
+val _ = export_rewrites ["swapstr_identity"]
+
+val swapstr_rewrites = store_thm(
+  "swapstr_rewrites",
+  ``(swapstr x y y = x) /\ (swapstr x y x = y)``,
+  SRW_TAC [][swapstr_def]);
+val _ = export_rewrites ["swapstr_rewrites"]
+
 
 
 
@@ -130,8 +159,6 @@ val swapset_11 = store_thm(
   METIS_TAC [swapstr_inverse]);
 val _ = export_rewrites ["swapset_11"]
 
-
-
 (* ----------------------------------------------------------------------
     Swapping over terms
    ---------------------------------------------------------------------- *)
@@ -167,7 +194,7 @@ val swap_comm = store_thm(
   HO_MATCH_MP_TAC nc_INDUCTION THEN SRW_TAC [][swap_def] THEN
   POP_ASSUM (Q.SPEC_THEN `NEW ({x;y} UNION (FV t DELETE x'))` SUBST1_TAC) THEN
   Q_TAC SUFF_TAC `{x;y} = {y;x}` THEN1 PROVE_TAC [] THEN
-  SRW_TAC [][pred_setTheory.EXTENSION] THEN PROVE_TAC []);
+  SRW_TAC [][EXTENSION] THEN PROVE_TAC []);
 
 val fresh_var_swap = store_thm(
   "fresh_var_swap",
@@ -201,11 +228,11 @@ val FV_swap = store_thm(
       `~(w = x)` by PROVE_TAC [] THEN
       SRW_TAC [][swapset_UNION] THEN
       `swapstr u v w = w` by SRW_TAC [][swapstr_def] THEN
-      SRW_TAC [][dBTheory.UNION_DELETE, pred_setTheory.SING_DELETE] THEN
-      SRW_TAC [][GSYM pred_setTheory.DELETE_NON_ELEMENT],
+      SRW_TAC [][dBTheory.UNION_DELETE, SING_DELETE] THEN
+      SRW_TAC [][GSYM DELETE_NON_ELEMENT],
       `FV t DELETE x = FV t`
-         by SRW_TAC [][GSYM pred_setTheory.DELETE_NON_ELEMENT] THEN
-      SRW_TAC [][GSYM pred_setTheory.DELETE_NON_ELEMENT, swapstr_def]
+         by SRW_TAC [][GSYM DELETE_NON_ELEMENT] THEN
+      SRW_TAC [][GSYM DELETE_NON_ELEMENT, swapstr_def]
     ],
     SRW_TAC [][lemma14a, EXTENSION, EQ_IMP_THM] THENL [
       SRW_TAC [][swapstr_def],
@@ -251,8 +278,6 @@ val swap_vsubst = store_thm(
       by (CONV_TAC (LAND_CONV (REWRITE_CONV [swap_def])) THEN
           NEW_ELIM_TAC THEN Q.X_GEN_TAC `a` THEN
           STRIP_TAC THENL [
-            `(swapstr u v' a = a) /\ (swapstr u v' z = z)`
-                by SRW_TAC [][swapstr_def] THEN
             ASM_SIMP_TAC (srw_ss()) [] THEN
             Q.ABBREV_TAC `uv'x = swapstr u v' x` THEN
             Q.ABBREV_TAC `uv'y = swapstr u v' y` THEN
@@ -267,16 +292,13 @@ val swap_vsubst = store_thm(
     POP_ASSUM SUBST_ALL_TAC THEN
     ASM_SIMP_TAC (srw_ss()) [swap_def] THEN NEW_ELIM_TAC THEN
     Q.X_GEN_TAC `a` THEN STRIP_TAC THENL [
-      `(swapstr u v' a = a) /\ (swapstr u v' z = z)`
-          by SRW_TAC [][swapstr_def] THEN
-      ASM_SIMP_TAC (srw_ss()) [] THEN
       `~(a IN FV (swap u v' M))` by ASM_SIMP_TAC (srw_ss()) [] THEN
       ASM_SIMP_TAC (srw_ss())[GSYM SIMPLE_ALPHA] THEN
       MATCH_MP_TAC (GSYM (last (CONJUNCTS SUB_THM))) THEN
-      SRW_TAC [][swapstr_def],
+      SRW_TAC [][],
       ASM_SIMP_TAC (srw_ss()) [lemma14a] THEN
       MATCH_MP_TAC (GSYM (last (CONJUNCTS SUB_THM))) THEN
-      SRW_TAC [][swapstr_def]
+      SRW_TAC [][]
     ]
   ]);
 
@@ -285,14 +307,9 @@ val swap_LAM = prove(
   SRW_TAC [][swap_def] THEN NEW_ELIM_TAC THEN Q.X_GEN_TAC `a` THEN
   STRIP_TAC THENL [
     SRW_TAC [][swap_vsubst] THEN
-    `swapstr x y a = a` by SRW_TAC [][swapstr_def] THEN
-    SRW_TAC [][] THEN
     MATCH_MP_TAC (GSYM SIMPLE_ALPHA) THEN
-    SRW_TAC [][swapset_def] THEN
-    Q_TAC SUFF_TAC `!z. (swapstr x y z = a) ==> (z = a)`
-      THEN1 METIS_TAC [] THEN
-    SRW_TAC [][swapstr_def],
-    SRW_TAC [][lemma14a, swapstr_def]
+    SRW_TAC [][],
+    SRW_TAC [][lemma14a]
   ]);
 
 val swap_thm = store_thm(
@@ -305,16 +322,25 @@ val swap_thm = store_thm(
 
 val swap_swap = store_thm(
   "swap_swap",
-  ``!t u v x y. swap x y (swap u v t) =
-                swap (swapstr x y u) (swapstr x y v) (swap x y t)``,
+  ``!t u v x y. swap (swapstr x y u) (swapstr x y v) (swap x y t) =
+                swap x y (swap u v t)``,
   HO_MATCH_MP_TAC nc_INDUCTION THEN REPEAT CONJ_TAC THENL [
     SRW_TAC [][swap_thm],
-    SRW_TAC [][swap_thm, SYM swapstr_swapstr],
+    SRW_TAC [][swap_thm],
     REPEAT STRIP_TAC THEN SIMP_TAC (srw_ss()) [swap_thm] THEN
     CONJ_TAC THEN FIRST_ASSUM MATCH_ACCEPT_TAC,
-    SRW_TAC [][swap_thm, SYM swapstr_swapstr] THEN
+    SRW_TAC [][swap_thm] THEN
     METIS_TAC [lemma14a]
   ]);
+val _ = export_rewrites ["swap_swap"]
+
+val swap_swap2 = store_thm(
+  "swap_swap2",
+  ``swap x y (swap (swapstr x y a) (swapstr x y b) t) =
+    swap a b (swap x y t)``,
+  CONV_TAC (LAND_CONV (ONCE_REWRITE_CONV [GSYM swap_swap])) THEN
+  REWRITE_TAC [swapstr_inverse]);
+val _ = export_rewrites ["swap_swap2"]
 
 val swap_inverse_lemma = prove(
   ``!t. swap x y (swap x y t) = t``,
@@ -326,23 +352,27 @@ val swap_inverse = store_thm(
   METIS_TAC [swap_inverse_lemma, swap_comm]);
 val _ = export_rewrites ["swap_inverse"]
 
+val swap_ALPHA = store_thm(
+  "swap_ALPHA",
+  ``~(v IN FV M) ==> (LAM v (swap v u M) = LAM u M)``,
+  SRW_TAC [][GSYM fresh_var_swap, GSYM SIMPLE_ALPHA]);
 
 val swap_subst = store_thm(
   "swap_subst",
-  ``!M. swap x y ([N/v] M) = [swap x y N / swapstr x y v] (swap x y M)``,
+  ``!M N v x y.
+      swap x y ([N/v] M) = [swap x y N / swapstr x y v] (swap x y M)``,
   HO_MATCH_MP_TAC pvh_induction THEN REPEAT STRIP_TAC THENL [
     SRW_TAC [][SUB_VAR, swap_thm],
     SRW_TAC [][SUB_THM, swap_thm],
     SRW_TAC [][SUB_THM, swap_thm],
     Q_TAC (NEW_TAC "z") `{v; v'; x; y} UNION FV M UNION FV N` THEN
-    `LAM v' M = LAM z ([VAR z/v'] M)` by SRW_TAC [][ALPHA] THEN
-    Q.ABBREV_TAC `M' = [VAR z/v'] M` THEN
+    `LAM v M = LAM z ([VAR z/v] M)` by SRW_TAC [][ALPHA] THEN
+    Q.ABBREV_TAC `M' = [VAR z/v] M` THEN
     `size M' = size M` by SRW_TAC [][] THEN
     ASM_SIMP_TAC (srw_ss()) [SUB_THM] THEN
     ASM_SIMP_TAC (srw_ss()) [swap_thm] THEN
-    `swapstr x y z = z` by SRW_TAC [][swapstr_def] THEN
-    `~(z IN FV (swap x y N))` by SRW_TAC [][FV_swap] THEN
-    `~(swapstr x y v = z)` by SRW_TAC [][swapstr_def] THEN
+    `~(z IN FV (swap x y N))` by SRW_TAC [][] THEN
+    `~(swapstr x y v = z)` by SRW_TAC [][] THEN
     ASM_SIMP_TAC (srw_ss()) [SUB_THM]
   ]);
 
@@ -376,55 +406,15 @@ val swap_11 = store_thm(
       FIRST_X_ASSUM (MP_TAC o MATCH_MP INJECTIVITY_LEMMA1) THEN
       DISCH_THEN SUBST_ALL_TAC THEN
       SRW_TAC [][fresh_var_swap] THEN
-      ONCE_REWRITE_TAC [swap_swap] THEN
-      `~(swapstr x y v IN FV (swap x y u))` by SRW_TAC [][FV_swap] THEN
+      ONCE_REWRITE_TAC [GSYM swap_swap] THEN
       SRW_TAC [][GSYM fresh_var_swap, SIMPLE_ALPHA]
     ]
   ]);
 val _ = export_rewrites ["swap_11"]
 
-(* swap moving over/around other functions *)
-val swap_rator = store_thm(
-  "swap_rator",
-  ``is_comb t ==> (rator (swap x y t) = swap x y (rator t))``,
-  Q.SPEC_THEN `t` STRUCT_CASES_TAC nc_CASES THEN
-  SRW_TAC [][swap_thm]);
-val _ = export_rewrites ["swap_rator"]
-
-val swap_rand = store_thm(
-  "swap_rand",
-  ``is_comb t ==> (rand (swap x y t) = swap x y (rand t))``,
-  Q.SPEC_THEN `t` STRUCT_CASES_TAC nc_CASES THEN
-  SRW_TAC [][swap_thm]);
-val _ = export_rewrites ["swap_rand"]
-
-val swap_is_comb = store_thm(
-  "swap_is_comb",
-  ``is_comb (swap x y t) = is_comb t``,
-  Q.SPEC_THEN `t` STRUCT_CASES_TAC nc_CASES THEN
-  SRW_TAC [][swap_thm]);
-val _ = export_rewrites ["swap_is_comb"]
-
-val swap_is_const = store_thm(
-  "swap_is_const",
-  ``is_const (swap x y t) = is_const t``,
-  Q.SPEC_THEN `t` STRUCT_CASES_TAC nc_CASES THEN
-  SRW_TAC [][swap_thm, is_const_thm]);
-val _ = export_rewrites ["swap_is_const"]
-
-val swap_dest_const = store_thm(
-  "swap_dest_const",
-  ``is_const t ==> (dest_const (swap x y t) = dest_const t)``,
-  Q.SPEC_THEN `t` STRUCT_CASES_TAC nc_CASES THEN
-  SRW_TAC [][swap_thm, is_const_thm]);
-val _ = export_rewrites ["swap_dest_const"]
-
-val swap_is_const2 = store_thm(
-  "swap_is_const2",
-  ``is_const t ==> (swap x y t = t)``,
-  Q.SPEC_THEN `t` STRUCT_CASES_TAC nc_CASES THEN
-  SRW_TAC [][swap_thm, is_const_thm]);
-val _ = export_rewrites ["swap_is_const2"]
+(* ----------------------------------------------------------------------
+    supporting recursion over lambda calculus terms using swap
+   ---------------------------------------------------------------------- *)
 
 val fresh_new_subst0 = prove(
   ``FINITE X ==>
@@ -434,61 +424,84 @@ val fresh_new_subst0 = prove(
   SRW_TAC [][fresh_var_swap, lemma14a]);
 
 val fresh_new_subst =
-    (SIMP_RULE bool_ss [pred_setTheory.FINITE_EMPTY,
-                        pred_setTheory.UNION_EMPTY] o
+    (SIMP_RULE bool_ss [FINITE_EMPTY,
+                        UNION_EMPTY] o
      Q.INST [`f` |-> `\v t. lam (hom t : 'b) v t  : 'b`,
              `X` |-> `EMPTY`] o
      INST_TYPE [alpha |-> beta, beta |-> alpha]) fresh_new_subst0
 
 
 val lemma =
-    (SIMP_RULE bool_ss [ABS_DEF, fresh_new_subst] o
+    (SIMP_RULE bool_ss [ASSUME ``FINITE (X:string set)``,
+                        ABS_DEF, fresh_new_subst0] o
      Q.INST [`lam` |->
-              `\r t. let v = NEW (FV (ABS t)) in lam (r v) v (t v) `] o
+              `\r t. let v = NEW (FV (ABS t) UNION X) in lam (r v) v (t v) `] o
      SPEC_ALL) nc_RECURSION
 
 val LET_RAND' = prove(
   ``(let x = M in P (N x)) = P (let x = M in N x)``,
   SRW_TAC [][]);
 
-val swap_RECURSION_term_out = store_thm(
-  "swap_RECURSION_term_out",
-  ``(!k. FV (con k) = {}) /\
-    (!s. FV (var s) SUBSET {s}) /\
-    (!t' u' t u. FV t' SUBSET FV t /\ FV u' SUBSET FV u ==>
-                 FV (app t' u' t u) SUBSET (FV t UNION FV u)) /\
-    (!t' v t. FV t' SUBSET FV t ==> FV (lam t' v t) SUBSET (FV (LAM v t))) /\
-    (!k x y. swap x y (con k) = con k) /\
-    (!s x y. swap x y (var s) = var (swapstr x y  s)) /\
+val swapping_def = Define`
+  swapping f fv =
+    (!x z. f x x z = z) /\
+    (!x y u v z. f x y (f u v z) =
+                   f (swapstr x y u) (swapstr x y v) (f x y z)) /\
+    (!x y z. f x y (f x y z) = z) /\
+    (!x y z z'. (f x y z = f x y z') = (z = z')) /\
+    (!x y z. ~(x IN fv z) /\ ~(y IN fv z) ==> (f x y z = z))
+`
+
+val LET_NEW_congruence = store_thm(
+  "LET_NEW_congruence",
+  ``(X = Y:string set) ==> FINITE Y ==> (!v. ~(v IN Y) ==> (P v = Q v)) ==>
+    (LET P (NEW X)  = LET Q (NEW Y))``,
+  SRW_TAC [][] THEN NEW_ELIM_TAC THEN SRW_TAC [][]);
+
+val swap_RECURSION_generic = store_thm(
+  "swap_RECURSION_generic",
+  ``swapping rswap rFV /\
+    FINITE X /\
+    (!k. rFV (con k) SUBSET X) /\
+    (!s. rFV (var s) SUBSET (s INSERT X)) /\
+    (!t' u' t u. rFV t' SUBSET (FV t UNION X) /\
+                 rFV u' SUBSET (FV u UNION X) ==>
+                 rFV (app t' u' t u) SUBSET FV (t @@ u) UNION X) /\
+    (!t' v t. rFV t' SUBSET (FV t UNION X) ==>
+              rFV (lam t' v t) SUBSET (FV (LAM v t) UNION X)) /\
+    (!k x y. ~(x IN X) /\ ~(y IN X) ==> (rswap x y (con k) = con k)) /\
+    (!s x y. ~(x IN X) /\ ~(y IN X) ==>
+             (rswap x y (var s) = var (swapstr x y  s))) /\
     (!t t' u u' x y.
-         swap x y (app t' u' t u) =
-         app (swap x y t') (swap x y u') (swap x y t) (swap x y u)) /\
+         ~(x IN X) /\ ~(y IN X) ==>
+         (rswap x y (app t' u' t u) =
+          app (rswap x y t') (rswap x y u') (swap x y t) (swap x y u))) /\
     (!t' t x y v.
-         swap x y (lam t' v t) =
-         lam (swap x y t') (swapstr x y v) (swap x y t)) ==>
-    ?hom.
-      (!t x y. hom (swap x y t) = swap x y (hom t)) /\
-      (!t. FV (hom t) SUBSET FV t) /\
-      (!k. hom (CON k) = con k) /\
-      (!s. hom (VAR s) = var s) /\
-      (!t u. hom (t @@ u) = app (hom t) (hom u) t u) /\
-      (!v t. hom (LAM v t) = lam (hom t) v t)``,
-  STRIP_TAC THEN
+         ~(x IN X) /\ ~(y IN X) ==>
+         (rswap x y (lam t' v t) =
+          lam (rswap x y t') (swapstr x y v) (swap x y t))) ==>
+    ?hom : 'a nc -> 'b.
+      ((!k. hom (CON k) = con k) /\
+       (!s. hom (VAR s) = var s) /\
+       (!t u. hom (t @@ u) = app (hom t) (hom u) t u) /\
+       (!v t. ~(v IN X) ==> (hom (LAM v t) = lam (hom t) v t))) /\
+      (!t x y. ~(x IN X) /\ ~(y IN X) ==>
+               (hom (swap x y t) = rswap x y (hom t))) /\
+      (!t. rFV (hom t) SUBSET FV t UNION X)``,
+  SRW_TAC [][swapping_def] THEN
   STRIP_ASSUME_TAC
-    (CONJUNCT1 (INST_TYPE [beta |-> ``:'b nc``]
-                          (CONV_RULE EXISTS_UNIQUE_CONV lemma))) THEN
+    (CONJUNCT1 (CONV_RULE EXISTS_UNIQUE_CONV lemma)) THEN
   Q.EXISTS_TAC `hom` THEN
   ASM_SIMP_TAC bool_ss [] THEN
-  `!t. FV (hom t) SUBSET FV t`
+  `!t. rFV (hom t) SUBSET FV t UNION X`
      by (HO_MATCH_MP_TAC nc_INDUCTION THEN
          ASM_SIMP_TAC (srw_ss()) [GSYM INSERT_SING_UNION] THEN
          REPEAT STRIP_TAC THEN
          NEW_ELIM_TAC THEN SRW_TAC [][] THENL [
-           MATCH_MP_TAC pred_setTheory.SUBSET_TRANS THEN
-           Q.EXISTS_TAC `FV (LAM v (swap v x t))` THEN
+           MATCH_MP_TAC SUBSET_TRANS THEN
+           Q.EXISTS_TAC `FV (LAM v (swap v x t)) UNION X` THEN
            CONJ_TAC THENL [
-             FIRST_X_ASSUM MATCH_MP_TAC THEN
-             ASM_SIMP_TAC bool_ss [GSYM fresh_var_swap],
+             ASM_SIMP_TAC bool_ss [FV_THM, GSYM fresh_var_swap],
              `LAM v (swap v x t) = LAM x t`
                 by ASM_SIMP_TAC bool_ss
                                 [GSYM fresh_var_swap, SIMPLE_ALPHA] THEN
@@ -497,107 +510,122 @@ val swap_RECURSION_term_out = store_thm(
            FULL_SIMP_TAC (srw_ss()) [] THEN
            FIRST_X_ASSUM MATCH_MP_TAC THEN METIS_TAC [lemma14a]
          ]) THEN
-  ASM_REWRITE_TAC [] THEN
-  `!v' v t u. lam (swap v' v t) v' (swap v' v u) =
-              lam (swap v' v t) (swapstr v' v v) (swap v' v u)`
-      by SIMP_TAC (srw_ss()) [swapstr_def] THEN
-  Q.PAT_ASSUM `!u w x y v. swap x y (lam u v w) = Z` (ASSUME_TAC o GSYM) THEN
-  `!t x y. hom (swap x y t) = swap x y (hom t)`
+  ASM_SIMP_TAC bool_ss [] THEN
+  Q.PAT_ASSUM `!u w x y v.
+                  P ==> (rswap x y (lam u v w) = Z)` (ASSUME_TAC o GSYM) THEN
+  `!t' t x y v.
+      ~(x IN X) /\ ~(y IN X) ==>
+      (lam (rswap x y t') v (swap x y t) =
+       rswap x y (lam t' (swapstr x y v) t))`
+    by PROVE_TAC [swapstr_inverse] THEN
+  Q.PAT_ASSUM `!x y u v z. rswap x y (rswap u v z) = Z`
+              (ASSUME_TAC o GSYM) THEN
+  `!t x y. ~(x IN X) /\ ~(y IN X) ==> (hom (swap x y t) = rswap x y (hom t))`
     by (HO_MATCH_MP_TAC pvh_induction THEN REPEAT CONJ_TAC THEN
         TRY (SRW_TAC [][swap_thm] THEN NO_TAC) THEN
         REPEAT STRIP_TAC THEN
-        ASM_SIMP_TAC bool_ss [swap_thm, size_swap] THEN
-        `!x y z u t. swap x (swapstr y z u) (swap y z (t:'b nc)) =
-                     swap y z (swap (swapstr y z x) u t)`
-            by (REPEAT GEN_TAC THEN
-                CONV_TAC (RAND_CONV (ONCE_REWRITE_CONV [swap_swap])) THEN
-                SRW_TAC [][]) THEN
-        ASM_SIMP_TAC bool_ss [] THEN
-        CONV_TAC (LAND_CONV (HO_REWR_CONV LET_RAND')) THEN
-        REWRITE_TAC [swap_11] THEN
-        `~(v IN FV (lam (hom t) v t))`
-             by (STRIP_TAC THEN
-                 `v IN FV (LAM v t)`
-                    by METIS_TAC [pred_setTheory.SUBSET_DEF] THEN
-                 POP_ASSUM MP_TAC THEN SRW_TAC[][]) THEN
-        `(let v' = NEW (FV (LAM v t)) in swap v' v (lam (hom t) v t)) =
-         lam (hom t) v t`
-            by (NEW_ELIM_TAC THEN SRW_TAC [][] THENL [
-                  `~(v' IN FV (lam (hom t) v t))`
-                       by (STRIP_TAC THEN
-                           `v' IN (FV (LAM v t))`
-                               by METIS_TAC [pred_setTheory.SUBSET_DEF] THEN
-                           POP_ASSUM MP_TAC THEN SRW_TAC [][]) THEN
-                  SRW_TAC [][GSYM fresh_var_swap, lemma14b],
-                  SRW_TAC [][]
-                ]) THEN
+        Cases_on `x = y` THEN1 SRW_TAC [][] THEN
+        `?z. ~(z IN {v;x;y} UNION X UNION FV t)`
+            by SRW_TAC [][dBTheory.FRESH_string] THEN
+        POP_ASSUM (STRIP_ASSUME_TAC o SIMP_RULE (srw_ss()) []) THEN
+        `LAM v t = LAM z ([VAR z/v] t)` by SRW_TAC [][SIMPLE_ALPHA] THEN
+        Q.ABBREV_TAC `M = [VAR z/v] t` THEN
+        `size t = size M` by SRW_TAC [][] THEN
+        POP_ASSUM SUBST_ALL_TAC THEN POP_ASSUM (K ALL_TAC) THEN
         POP_ASSUM SUBST_ALL_TAC THEN
-        NEW_ELIM_TAC THEN SRW_TAC [][] THENL [
-          Q_TAC SUFF_TAC `~(swapstr x y v' IN FV (lam (hom t) v t))` THEN1
-                SRW_TAC [][GSYM fresh_var_swap, lemma14b] THEN
-          STRIP_TAC THEN
-          `swapstr x y v' IN FV (LAM v t)`
-              by METIS_TAC [pred_setTheory.SUBSET_DEF] THEN
-          POP_ASSUM MP_TAC THEN SRW_TAC [][] ,
-          SRW_TAC [][]
+        `hom (swap x y (LAM z M)) = rswap x y (lam (hom M) z M)`
+          by (ASM_SIMP_TAC bool_ss [swap_thm, swapstr_def] THEN
+              NEW_ELIM_TAC THEN ASM_REWRITE_TAC [] THEN
+              Q.X_GEN_TAC `a` THEN REVERSE (SRW_TAC [][]) THEN1
+                ASM_SIMP_TAC bool_ss [swapstr_def] THEN
+              Q.ABBREV_TAC `N = lam (hom M) z M` THEN
+              `rswap a z (rswap x y N) =
+                 rswap x y (rswap x y (rswap a z (rswap x y N)))`
+                    by SRW_TAC [][] THEN
+              ` _ = rswap x y (rswap (swapstr x y a) (swapstr x y z)
+                                     (rswap x y (rswap x y N)))`
+                    by SRW_TAC [][] THEN
+              ` _ = rswap x y (rswap (swapstr x y a) (swapstr x y z) N)`
+                    by SRW_TAC [][] THEN
+              SRW_TAC [][] THEN
+              FIRST_X_ASSUM MATCH_MP_TAC THEN
+              `rFV (lam (hom M) z M) SUBSET FV M DELETE z UNION X`
+                 by METIS_TAC [] THEN
+              REPEAT STRIP_TAC THENL [
+                `swapstr x y a IN FV M DELETE z UNION X`
+                    by PROVE_TAC [SUBSET_DEF] THEN
+                POP_ASSUM MP_TAC THEN SRW_TAC [][] THEN
+                SRW_TAC [][swapstr_def],
+                `z IN FV M DELETE z UNION X`
+                    by PROVE_TAC [SUBSET_DEF] THEN
+                POP_ASSUM MP_TAC THEN SRW_TAC [][]
+              ]) THEN
+        POP_ASSUM SUBST_ALL_TAC THEN ASM_SIMP_TAC bool_ss [] THEN
+        NEW_ELIM_TAC THEN ASM_REWRITE_TAC [] THEN Q.X_GEN_TAC `a` THEN
+        REVERSE (SRW_TAC [][]) THEN1 SRW_TAC [][] THEN
+        Q_TAC SUFF_TAC
+          `~(a IN rFV (lam (hom M) z M)) /\ ~(z IN rFV (lam (hom M) z M))`
+              THEN1 PROVE_TAC [] THEN
+        `rFV (lam (hom M) z M) SUBSET FV M DELETE z UNION X`
+           by PROVE_TAC [] THEN
+        REPEAT STRIP_TAC THENL [
+          `a IN FV M DELETE z UNION X` by PROVE_TAC [SUBSET_DEF] THEN
+          POP_ASSUM MP_TAC THEN SRW_TAC [][],
+          `z IN FV M DELETE z UNION X` by PROVE_TAC [SUBSET_DEF] THEN
+          POP_ASSUM MP_TAC THEN SRW_TAC [][]
         ]) THEN
   ASM_SIMP_TAC bool_ss [] THEN
-  REPEAT GEN_TAC THEN NEW_ELIM_TAC THEN SRW_TAC [][] THENL [
-    Q_TAC SUFF_TAC `~(v' IN FV (lam (hom t) v t)) /\
-                    ~(v IN FV (lam (hom t) v t))` THEN1
-          SRW_TAC [][GSYM fresh_var_swap, lemma14b] THEN
-    REPEAT STRIP_TAC THENL [
-      `v' IN FV (LAM v t)` by METIS_TAC [pred_setTheory.SUBSET_DEF] THEN
-      FULL_SIMP_TAC (srw_ss()) [],
-      `v IN FV (LAM v t)` by METIS_TAC [pred_setTheory.SUBSET_DEF] THEN
-      FULL_SIMP_TAC (srw_ss()) []
-    ],
+  REPEAT GEN_TAC THEN STRIP_TAC THEN NEW_ELIM_TAC THEN SRW_TAC [][] THENL [
+    Cases_on `v = v'` THEN1 SRW_TAC [][] THEN
+    SRW_TAC [][] THEN
+    Q_TAC SUFF_TAC `~(v' IN rFV (lam (hom t) v t)) /\
+                    ~(v IN rFV (lam (hom t) v t))` THEN1
+          SRW_TAC [][] THEN
+    PROVE_TAC [SUBSET_DEF, IN_DELETE, IN_UNION],
     SRW_TAC [][]
   ]);
 
-val swap_RECURSION = store_thm(
-  "swap_RECURSION",
-  ``(!s x y. var (swapstr x y s) = var s) /\
-    (!t t' u u' x y.
-       app t' u' (swap x y t) (swap x y u) =
-       app t' u' t u) /\
-    (!t' t x y v.
-       lam t' (swapstr x y v) (swap x y t) = lam t' v t) ==>
-    ?hom : 'a nc -> 'b.
-      (!t x y. hom (swap x y t) = hom t) /\
-      (!k. hom (CON k) = con k) /\
-      (!s. hom (VAR s) = var s) /\
-      (!t u. hom (t @@ u) = app (hom t) (hom u) t u) /\
-      (!v t. hom (LAM v t) = lam (hom t) v t)``,
-  STRIP_TAC THEN
-  STRIP_ASSUME_TAC
-    (CONJUNCT1 (CONV_RULE EXISTS_UNIQUE_CONV lemma)) THEN
-  Q.EXISTS_TAC `hom` THEN ASM_REWRITE_TAC [] THEN
-  `!t x y. hom (swap x y t) = hom t`
-     by (HO_MATCH_MP_TAC pvh_induction THEN
-         REPEAT STRIP_TAC THEN TRY (SRW_TAC [][swap_thm] THEN NO_TAC) THEN
-         `hom (LAM v t) = let u = NEW (FV (LAM v t)) in
-                            lam (hom (swap u v t)) u (swap u v t)`
-            by SRW_TAC [][] THEN
-         ` _ = let u = NEW (FV (LAM v t)) in
-                         lam (hom (swap u v t)) (swapstr u v v) (swap u v t)`
-            by SIMP_TAC bool_ss [swapstr_def] THEN
-         ` _ = let u = NEW (FV (LAM v t)) in lam (hom t) v t`
-            by SRW_TAC [][] THEN
-         ` _ = lam (hom t) v t` by SRW_TAC [][] THEN
-         POP_ASSUM SUBST_ALL_TAC THEN
-         ASM_SIMP_TAC bool_ss [swap_thm] THEN
-         `!u v t t'. lam (hom (swap u v t)) u (swap u v t') =
-                     lam (hom (swap u v t)) (swapstr u v v) (swap u v t')`
-            by SIMP_TAC bool_ss [swapstr_def] THEN
-         ASM_SIMP_TAC bool_ss [size_swap] THEN
-         SRW_TAC [][]) THEN
-  ASM_REWRITE_TAC [] THEN REPEAT GEN_TAC THEN
-  `!v'. lam (hom t) v' (swap v' v t) =
-        lam (hom t) (swapstr v' v v) (swap v' v t)`
-      by SIMP_TAC (srw_ss()) [swapstr_def] THEN
-  ASM_SIMP_TAC bool_ss [] THEN SRW_TAC [][]);
+val swap_RECURSION_nosideset = save_thm(
+  "swap_RECURSION_nosideset",
+  SIMP_RULE (srw_ss()) [] (Q.INST [`X` |-> `{}`] swap_RECURSION_generic));
 
+val null_swapping = store_thm(
+  "null_swapping",
+  ``swapping (\x y z. z) (\z. {})``,
+  SRW_TAC [][swapping_def]);
+
+val swap_identity = store_thm(
+  "swap_identity",
+  ``!t x y. ~(x IN FV t) /\ ~(y IN FV t) ==> (swap x y t = t)``,
+  HO_MATCH_MP_TAC nc_INDUCTION THEN SIMP_TAC (srw_ss()) [swap_thm] THEN
+  MAP_EVERY Q.X_GEN_TAC [`v`, `t`] THEN STRIP_TAC THEN
+  MAP_EVERY Q.X_GEN_TAC [`x`, `y`] THEN STRIP_TAC THENL [
+    `swap x y t = t` by METIS_TAC [lemma14a] THEN
+    Cases_on `v = x` THEN SRW_TAC [][swapstr_def] THEN
+    MATCH_MP_TAC INJECTIVITY_LEMMA3 THEN Q.EXISTS_TAC `v` THEN
+    SRW_TAC [][lemma14b],
+    SRW_TAC [][] THEN METIS_TAC [swap_ALPHA, swap_comm],
+    SRW_TAC [][] THEN METIS_TAC [swap_ALPHA, swap_comm],
+    SRW_TAC [][]
+  ]);
+
+val nc_swapping = store_thm(
+  "nc_swapping",
+  ``swapping swap FV``,
+  SIMP_TAC (srw_ss()) [swap_swap, swapping_def, swap_identity]);
+
+val swapping_implies_empty_swap = store_thm(
+  "swapping_implies_empty_swap",
+  ``swapping sw fv /\ (fv t = {}) ==> !x y. sw x y t = t``,
+  SRW_TAC [][swapping_def]);
+
+
+
+val swap_RECURSION_simple = save_thm(
+  "swap_RECURSION_simple",
+  (SIMP_RULE (srw_ss()) [null_swapping] o
+   Q.INST [`rswap` |-> `\x y z. z`, `rFV` |-> `\z. {}`])
+    swap_RECURSION_nosideset);
 
 (* examples
 
